prove c_kp54_evp.

Computability/Constructions/KP54.lean
@@ -12,11 +12,14 @@ section kp54
 
 -- theorem c_kp54_ev : eval (K0 Nat.fzero) c_kp54 = KP54 := by sorry
 
-@[irreducible] noncomputable def c_c_kp54_aux (i n:ℕ) :=
+def c_c_kp54_aux :=
   zero
--- theorem c_c_kp54_aux_evp : 
+@[simp] theorem c_c_kp54_aux_evp : eval_prim O c_c_kp54_aux (Nat.pair i n) = dovetail (KP54.c_kp54_aux i n) := by sorry
+def c_c_evals :=
+  zero
+@[simp] theorem c_c_evals_evp : eval_prim O c_c_evals x = c_evals := by sorry
 
-
+#check c_evals
 def c_kp54_main :=
   have s := left
   have KP54s := right
@@ -27,10 +30,27 @@ def c_kp54_main :=
   let la := c_list_length.comp Aₚ
   c_ifz.comp₃ (c_mod.comp₂ (succ.comp s) (c_const 2))
   (
-    let dvt := oracle.comp zero
-    c_eval
+    let q0 := oracle.comp₂ (c_c_kp54_aux.comp₂ i lb) Aₚ
+    c_ifz.comp₃ q0
+    (pair (c_list_concat.comp₂ Aₚ zero) (c_list_concat.comp₂ Bₚ zero))
+    (
+      let rf := left.comp (c_pred.comp q0)
+      let Aₛ := c_list_append.comp₂ Aₚ (succ.comp rf)
+      let A_result := c_pred.comp $ oracle.comp₂ c_c_evals (pair Aₛ (pair i lb))
+      pair Aₛ (c_list_concat.comp₂ Bₚ (c_sg'.comp A_result))
+    )
   )
-  c_evaln
+  (
+    let q0 := oracle.comp₂ (c_c_kp54_aux.comp₂ i la) Bₚ
+    c_ifz.comp₃ q0
+    (pair (c_list_concat.comp₂ Aₚ zero) (c_list_concat.comp₂ Bₚ zero))
+    (
+      let rf := left.comp (c_pred.comp q0)
+      let Bₛ := c_list_append.comp₂ Bₚ (succ.comp rf)
+      let B_result := c_pred.comp $ oracle.comp₂ c_c_evals (pair Bₛ (pair i la))
+      pair (c_list_concat.comp₂ Aₚ (c_sg'.comp B_result)) Bₛ
+    )
+  )
   -- c_eval
 def c_kp54 :=
   (
@@ -45,23 +65,98 @@ def c_kp54 :=
     simp [c_kp54]
     unfold KP54.KP54
     rfl
-  | succ x ih =>
+  | succ s_1 ih =>
     unfold c_kp54
     simp
-    have : (Nat.rec 0 (fun y IH ↦ eval_prim (K0 Nat.fzero) c_kp54_main (Nat.pair y IH)) x) = eval_prim (K0 Nat.fzero) c_kp54 x := by 
+    have : (Nat.rec 0 (fun y IH ↦ eval_prim (K0 Nat.fzero) c_kp54_main (Nat.pair y IH)) s_1) = eval_prim (K0 Nat.fzero) c_kp54 s_1 := by
       unfold c_kp54
-      cases x <;> simp
-    -- simp (config := {zeta:=false}) only []
-    rw [this, ih]; clear this ih
-    
+      cases s_1 <;> simp
+    -- we are careful with the rewriting/unfolding order here.
+    rewrite [this]; clear this
     unfold c_kp54_main
-    simp
-    rw (config:={occs:=.pos [1]}) [KP54.KP54]
-    simp (config := {zeta:=false}) []
+    lift_lets; extract_lets; expose_names
+    unfold KP54.KP54
+    rw [ih]; clear ih
+    lift_lets; extract_lets; expose_names
 
-    sorry
+    let (eq:=hinp) inp := (Nat.pair s_1 (KP54.KP54 s_1))
 
-  
+    have hs : eval_prim (K0 Nat.fzero) s inp = s_1 := by simp [s, inp]
+    have hi : eval_prim (K0 Nat.fzero) i inp = i_1 := by simp [i, i_1, hs]
+    have hKP54s : eval_prim (K0 Nat.fzero) KP54s inp = KP54.KP54 s_1 := by simp [KP54s, inp]
+    have hAₚ : eval_prim (K0 Nat.fzero) Aₚ inp = Aₚ_1 := by simp [Aₚ, Aₚ_1, hKP54s]
+    have hBₚ : eval_prim (K0 Nat.fzero) Bₚ inp = Bₚ_1 := by simp [Bₚ, Bₚ_1, hKP54s]
+    have hla : eval_prim (K0 Nat.fzero) la inp = la_1 := by simp [la, la_1, hAₚ]
+    have hlb : eval_prim (K0 Nat.fzero) lb inp = lb_1 := by simp [lb, lb_1, hBₚ]
+
+    simp (config := {zeta:=false}) [←hinp]
+    simp (config := {zeta:=false}) [hs]
+    split
+    next h0 =>
+      split
+      next h1 =>
+        have : ¬ dvt.Dom := by simp [q0, hi, hlb, hAₚ] at h1; exact h1
+        simp (config := {zeta:=false}) [this, hAₚ, hBₚ]
+      next h1 =>
+        have : dvt.Dom := by simp [q0, hi, hlb, hAₚ] at h1; exact h1
+        simp (config := {zeta:=false}) [this]
+        lift_lets; extract_lets; expose_names
+        have hrf : eval_prim (K0 Nat.fzero) rf inp = rf_2 := by
+          simp [rf, rf_2,q0]
+          split
+          next h2 => simp [hi, hlb, hAₚ]; congr
+          next h2 =>
+            simp [hi, hlb, hAₚ] at h2
+            simp [dvt, h2] at this
+        have hAₛ : eval_prim (K0 Nat.fzero) Aₛ inp = Aₛ_1 := by simp [Aₛ, Aₛ_1, hAₚ, hrf, -Denumerable.list_ofNat_succ]
+        have hA_result : eval_prim (K0 Nat.fzero) A_result inp = A_result_1 := by
+          simp [A_result, A_result_1]
+          split
+          next h2 => simp [hAₛ, hi, hlb]
+          next h2 =>
+            -- this case is a contradiction, as we know the evals must halt from "this".
+            simp [dvt] at this
+            simp [hAₛ, hi, hlb] at h2
+            have contra : (evals Aₛ_1 (decodeCode i_1) lb_1).Dom := by
+              have a0 := dovetail_ev_0' this
+              simp [KP54.c_kp54_aux_evp, -Denumerable.list_ofNat_succ] at a0
+              exact a0
+            simp [contra] at h2
+        simp [hAₛ, hBₚ, hA_result]
+    -- proof practically idential to above.
+    next h0 =>
+      split
+      next h1 =>
+        have : ¬ dvt_1.Dom := by simp [q0_1, hi, hla, hBₚ] at h1; exact h1
+        simp (config := {zeta:=false}) [this, hAₚ, hBₚ]
+      next h1 =>
+        have : dvt_1.Dom := by simp [q0_1, hi, hla, hBₚ] at h1; exact h1
+        simp (config := {zeta:=false}) [this]
+        lift_lets; extract_lets; expose_names
+        have hrf : eval_prim (K0 Nat.fzero) rf_1 inp = rf_2 := by
+          simp [rf_1, rf_2,q0_1]
+          split
+          next h2 => simp [hi]; congr
+          next h2 =>
+            simp [hi, hla, hBₚ] at h2
+            simp [dvt_1, h2] at this
+        have hBₛ : eval_prim (K0 Nat.fzero) Bₛ inp = Bₛ_1 := by simp [Bₛ, Bₛ_1, hBₚ, hrf, -Denumerable.list_ofNat_succ]
+        have hB_result : eval_prim (K0 Nat.fzero) B_result inp = B_result_1 := by
+          simp [B_result, B_result_1]
+          split
+          next h2 => simp [hBₛ, hi, hla]
+          next h2 =>
+            -- this case is a contradiction, as we know the evals must halt from "this".
+            simp [dvt_1] at this
+            simp [hBₛ, hi, hla] at h2
+            have contra : (evals Bₛ_1 (decodeCode i_1) la_1).Dom := by
+              have a0 := dovetail_ev_0' this
+              simp [KP54.c_kp54_aux_evp, -Denumerable.list_ofNat_succ] at a0
+              exact a0
+            simp [contra] at h2
+        simp [hBₛ, hAₚ, hB_result]
+
+
 -- theorem c_kp54_ev : (eval (∅⌜) c_kp54 x).get (c_kp54_t x) = KP54.KP54 x := by sorry
 
 section n2b
@@ -92,9 +187,9 @@ theorem c_kp54_A_evp : eval_prim (K0 Nat.fzero) c_kp54_A = χ KP54.A := by
   simp [χ]
   congr
   exact getI_eq_getElem
-  
-  
-  
+
+
+
 
 theorem A_le_J1 : KP54.A ≤ᵀ ∅⌜ := by
   unfold KP54.A
@@ -103,9 +198,9 @@ theorem A_le_J1 : KP54.A ≤ᵀ ∅⌜ := by
   simp
   unfold SetTuringReducible
   simp [SetTuringReducible]
-  
 
-  
+
+
   sorry
 
 -- end Nat.RecursiveIn.Code
